src/trans/SplitRelCommon.v
@@ -1,172 +1,204 @@
 From sflib Require Import sflib.
 From Paco Require Import paco.
 
+From PromisingLib Require Import Axioms.
 From PromisingLib Require Import Basic.
 From PromisingLib Require Import Loc.
+From PromisingLib Require Import DataStructure.
+From PromisingLib Require Import DenseOrder.
 From PromisingLib Require Import Language.
-
 From PromisingLib Require Import Event.
+
 Require Import Time.
 Require Import View.
+Require Import BoolMap.
+Require Import Promises.
 Require Import Cell.
 Require Import Memory.
+Require Import Global.
 Require Import TView.
 Require Import Local.
 Require Import Thread.
 Require Import Configuration.
 
-Require Import FulfillStep.
-
-Require Import SimMemory.
-Require Import SimPromises.
 Require Import SimLocal.
-Require Import SimThread.
+Require Import SimMemory.
+Require Import SimGlobal.
 
 Set Implicit Arguments.
 
 
 Lemma sim_local_fulfill_released
-      lc1_src sc1_src mem1_src
-      lc1_tgt sc1_tgt mem1_tgt
-      lc2_tgt sc2_tgt
-      loc from to val releasedm_src releasedm_tgt released
+      lc1_src gl1_src
+      lc1_tgt gl1_tgt
+      loc prm2 gprm2
+      (LOCAL1: sim_local lc1_src lc1_tgt)
+      (GLOBAL1: sim_global gl1_src gl1_tgt)
+      (FULFILL_TGT: Promises.fulfill lc1_tgt.(Local.promises) gl1_tgt.(Global.promises) loc Ordering.strong_relaxed prm2 gprm2):
+  Promises.fulfill lc1_src.(Local.promises) gl1_src.(Global.promises) loc Ordering.acqrel prm2 gprm2.
+Proof.
+  destruct lc1_src, lc1_tgt, gl1_src, gl1_tgt.
+  inv LOCAL1. inv GLOBAL1. ss. subst.
+  inv FULFILL_TGT; eauto.
+Qed.
+
+Lemma sim_local_write_released
+      lc1_src gl1_src
+      lc1_tgt gl1_tgt
+      lc2_tgt gl2_tgt
+      loc from to val releasedm_src releasedm_tgt released_tgt
       (RELM_LE: View.opt_le releasedm_src releasedm_tgt)
-      (RELM_WF: View.opt_wf releasedm_src)
-      (RELM_CLOSED: Memory.closed_opt_view releasedm_src mem1_src)
-      (WF_RELM_TGT: View.opt_wf releasedm_tgt)
-      (STEP_TGT: fulfill_step lc1_tgt sc1_tgt loc from to val releasedm_tgt released Ordering.strong_relaxed lc2_tgt sc2_tgt)
-      (LOCAL1: sim_local SimPromises.bot lc1_src lc1_tgt)
-      (RELEASED1: View.le (TView.cur (Local.tview lc1_tgt)) (View.join ((TView.rel (Local.tview lc1_tgt)) loc) (View.singleton_ur loc to)))
-      (SC1: TimeMap.le sc1_src sc1_tgt)
-      (MEM1: sim_memory mem1_src mem1_tgt)
-      (WF1_SRC: Local.wf lc1_src mem1_src)
-      (WF1_TGT: Local.wf lc1_tgt mem1_tgt)
-      (SC1_SRC: Memory.closed_timemap sc1_src mem1_src)
-      (SC1_TGT: Memory.closed_timemap sc1_tgt mem1_tgt)
-      (MEM1_SRC: Memory.closed mem1_src)
-      (MEM1_TGT: Memory.closed mem1_tgt):
-  exists lc2_src sc2_src,
-    <<STEP_SRC: fulfill_step lc1_src sc1_src loc from to val releasedm_src released Ordering.acqrel lc2_src sc2_src>> /\
-    <<LOCAL2: sim_local SimPromises.bot lc2_src lc2_tgt>> /\
-    <<SC2: TimeMap.le sc2_src sc2_tgt>>.
+      (RELM_WF_SRC: View.opt_wf releasedm_src)
+      (RELM_CLOSED_SRC: Memory.closed_opt_view releasedm_src (Global.memory gl1_src))
+      (RELM_WF_TGT: View.opt_wf releasedm_tgt)
+      (STEP_TGT: Local.write_step lc1_tgt gl1_tgt loc from to val releasedm_tgt released_tgt Ordering.strong_relaxed lc2_tgt gl2_tgt)
+      (LOCAL1: sim_local lc1_src lc1_tgt)
+      (GLOBAL1: sim_global gl1_src gl1_tgt)
+      (LC_WF1_SRC: Local.wf lc1_src gl1_src)
+      (LC_WF1_TGT: Local.wf lc1_tgt gl1_tgt)
+      (GL_WF1_SRC: Global.wf gl1_src)
+      (GL_WF1_TGT: Global.wf gl1_tgt)
+      (RELEASED1: View.le (TView.cur (Local.tview lc1_tgt))
+                          (View.join ((TView.rel (Local.tview lc1_tgt)) loc) (View.singleton_ur loc to))):
+  exists released_src lc2_src gl2_src,
+    <<STEP_SRC: Local.write_step lc1_src gl1_src loc from to val releasedm_src released_src Ordering.acqrel lc2_src gl2_src>> /\
+    <<REL: View.opt_le released_src released_tgt>> /\
+    <<LOCAL2: sim_local lc2_src lc2_tgt>> /\
+    <<GLOBAL2: sim_global gl2_src gl2_tgt>>.
 Proof.
   inv STEP_TGT.
-  assert (RELT_LE:
+  assert (REL:
    View.opt_le
-     (TView.write_released (Local.tview lc1_src) sc1_src loc to releasedm_src Ordering.acqrel)
-     (TView.write_released (Local.tview lc1_tgt) sc2_tgt loc to releasedm_tgt Ordering.strong_relaxed)).
+     (TView.write_released (Local.tview lc1_src) loc to releasedm_src Ordering.acqrel)
+     (TView.write_released (Local.tview lc1_tgt) loc to releasedm_tgt Ordering.strong_relaxed)).
   { unfold TView.write_released, TView.write_tview. ss. viewtac;
-      try econs; repeat (condtac; aggrtac); try apply WF1_TGT.
+      try econs; repeat (condtac; aggrtac); try apply LC_WF1_TGT.
     rewrite <- View.join_r. etrans; eauto. apply LOCAL1.
   }
-  assert (RELT_WF:
-   View.opt_wf (TView.write_released (Local.tview lc1_src) sc1_src loc to releasedm_src Ordering.acqrel)).
+  assert (REL_WF:
+   View.opt_wf (TView.write_released (Local.tview lc1_src) loc to releasedm_src Ordering.acqrel)).
   { unfold TView.write_released. condtac; econs.
-    repeat (try condtac; viewtac; try apply WF1_SRC).
+    repeat (try condtac; viewtac; try apply LC_WF1_SRC).
   }
-  exploit SimPromises.remove_bot; try exact REMOVE;
-    try exact MEM1; try apply LOCAL1; eauto.
-  i. des. esplits.
+  exploit sim_memory_add_exists; try exact WRITE; try apply GLOBAL1.
+  { econs 1. exact REL_WF. }
+  { econs; try exact REL; [refl|].
+    instantiate (1:=Ordering.le Ordering.acqrel Ordering.na).
+    refl.
+  }
+  i. des.
+  exploit sim_local_fulfill_released; try apply LOCAL1; eauto. i.
+  esplits.
   - econs; eauto.
     inv WRITABLE. econs; ss. eapply TimeFacts.le_lt_lt; [apply LOCAL1|apply TS].
-  - econs; eauto. s.
+  - ss.
+  - inv LOCAL1. econs; eauto. ss.
     unfold TView.write_tview, View.singleton_ur_if. repeat (condtac; aggrtac).
     econs; repeat (condtac; aggrtac);
       (try by etrans; [apply LOCAL1|aggrtac]);
       (try by rewrite <- ? View.join_r; econs; aggrtac);
-      (try apply WF1_TGT).
+      (try apply LC_WF1_TGT).
     + ss. i. unfold LocFun.find. repeat (condtac; aggrtac).
-      * etrans; eauto. apply LOCAL1.
-      * apply LOCAL1.
-    + ss. aggrtac; try apply WF1_TGT. rewrite <- ? View.join_l. apply LOCAL1.
-    + ss. aggrtac; try apply WF1_TGT. rewrite <- ? View.join_l. apply LOCAL1.
-  - ss.
+      * etrans; eauto. apply TVIEW.
+      * apply TVIEW.
+    + ss. aggrtac; try apply LC_WF1_TGT.
+      rewrite <- ? View.join_l. apply TVIEW.
+    + ss. aggrtac; try apply LC_WF1_TGT.
+      rewrite <- ? View.join_l. apply TVIEW.
+  - inv GLOBAL1. econs; ss.
 Qed.
 
-Lemma sim_local_write_released
-      lc1_src sc1_src mem1_src
-      lc1_tgt sc1_tgt mem1_tgt
-      lc2_tgt sc2_tgt mem2_tgt
-      loc from to val releasedm_src releasedm_tgt released_tgt kind
-      (RELM_LE: View.opt_le releasedm_src releasedm_tgt)
-      (RELM_SRC_WF: View.opt_wf releasedm_src)
-      (RELM_SRC_CLOSED: Memory.closed_opt_view releasedm_src mem1_src)
-      (RELM_TGT_WF: View.opt_wf releasedm_tgt)
-      (RELM_TGT_CLOSED: Memory.closed_opt_view releasedm_tgt mem1_tgt)
-      (STEP_TGT: Local.write_step lc1_tgt sc1_tgt mem1_tgt loc from to val releasedm_tgt released_tgt Ordering.strong_relaxed lc2_tgt sc2_tgt mem2_tgt kind)
-      (LOCAL1: sim_local SimPromises.bot lc1_src lc1_tgt)
-      (RELEASED1: View.le (TView.cur (Local.tview lc1_tgt)) (View.join ((TView.rel (Local.tview lc1_tgt)) loc) (View.singleton_ur loc to)))
-      (SC1: TimeMap.le sc1_src sc1_tgt)
-      (MEM1: sim_memory mem1_src mem1_tgt)
-      (WF1_SRC: Local.wf lc1_src mem1_src)
-      (WF1_TGT: Local.wf lc1_tgt mem1_tgt)
-      (SC1_SRC: Memory.closed_timemap sc1_src mem1_src)
-      (SC1_TGT: Memory.closed_timemap sc1_tgt mem1_tgt)
-      (MEM1_SRC: Memory.closed mem1_src)
-      (MEM1_TGT: Memory.closed mem1_tgt):
-  exists released_src lc2_src sc2_src mem2_src,
-    <<STEP_SRC: Local.write_step lc1_src sc1_src mem1_src loc from to val releasedm_src released_src Ordering.acqrel lc2_src sc2_src mem2_src kind>> /\
-    <<REL2: View.opt_le released_src released_tgt>> /\
-    <<LOCAL2: sim_local SimPromises.bot lc2_src lc2_tgt>> /\
-    <<SC2: TimeMap.le sc2_src sc2_tgt>> /\
-    <<MEM2: sim_memory mem2_src mem2_tgt>>.
+Lemma sim_local_update_released
+      lc1_src gl1_src
+      lc1_tgt gl1_tgt
+      lc2_tgt
+      lc3_tgt gl3_tgt
+      loc ts1 val1 released1_tgt ord1_src ord1_tgt
+      to2 val2 released2_tgt
+      (STEP1_TGT: Local.read_step lc1_tgt gl1_tgt loc ts1 val1 released1_tgt ord1_tgt lc2_tgt)
+      (STEP2_TGT: Local.write_step lc2_tgt gl1_tgt loc ts1 to2 val2 released1_tgt released2_tgt Ordering.strong_relaxed lc3_tgt gl3_tgt)
+      (ORD1: Ordering.le ord1_src ord1_tgt)
+      (ORD1_TGT: Ordering.le ord1_tgt Ordering.strong_relaxed)
+      (LOCAL1: sim_local lc1_src lc1_tgt)
+      (GLOBAL1: sim_global gl1_src gl1_tgt)
+      (LC_WF1_SRC: Local.wf lc1_src gl1_src)
+      (LC_WF1_TGT: Local.wf lc1_tgt gl1_tgt)
+      (GL_WF1_SRC: Global.wf gl1_src)
+      (GL_WF1_TGT: Global.wf gl1_tgt)
+      (RELEASED1: View.le (TView.cur (Local.tview lc1_tgt)) ((TView.rel (Local.tview lc1_tgt)) loc)):
+  exists released1_src released2_src lc2_src lc3_src gl3_src,
+    <<STEP1_SRC: Local.read_step lc1_src gl1_src loc ts1 val1 released1_src ord1_src lc2_src>> /\
+    <<STEP2_SRC: Local.write_step lc2_src gl1_src loc ts1 to2 val2 released1_src released2_src Ordering.acqrel lc3_src gl3_src>> /\
+    <<REL1: View.opt_le released1_src released1_tgt>> /\
+    <<REL2: View.opt_le released2_src released2_tgt>> /\
+    <<LOCAL3: sim_local lc3_src lc3_tgt>> /\
+    <<GLOBAL3: sim_global gl3_src gl3_tgt>>.
 Proof.
-  exploit write_promise_fulfill; eauto. i. des.
-  exploit Local.promise_step_future; eauto. i. des.
-  exploit sim_local_promise_bot; eauto. i. des.
-  exploit Local.promise_step_future; eauto. i. des.
-  exploit sim_local_fulfill_released; try apply STEP2;
-    try apply LOCAL2; try apply MEM2; eauto.
-  { eapply Memory.future_closed_opt_view; eauto. }
-  { by inv STEP1. }
-  i. des.
-  exploit promise_fulfill_write_sim_memory; try exact STEP_SRC; try exact STEP_SRC0; eauto.
-  { i. hexploit ORD; eauto. i. des. splits; ss.
-    eapply sim_local_nonsynch_loc; eauto.
+  exploit sim_local_read; try exact STEP1_TGT; eauto. i. des.
+  exploit Local.read_step_future; try exact STEP1_TGT; eauto. i. des.
+  exploit Local.read_step_future; try exact STEP_SRC; eauto. i. des.
+  exploit sim_local_write_released; try exact STEP2_TGT; eauto.
+  { inv STEP1_TGT. ss.
+    condtac; try by (destruct ord1_tgt; ss).
+    rewrite View.join_bot_r.
+    apply View.join_le; ss.
+    inv STEP2_TGT. exploit Memory.add_ts; eauto. i.
+    aggrtac. condtac; aggrtac.
   }
-  i. des. esplits; eauto. etrans; eauto.
+  i. des.
+  esplits; eauto.
+Qed.
+
+Lemma sim_local_is_racy_released
+      lc1_src gl1_src
+      lc1_tgt gl1_tgt
+      loc to
+      (STEP_TGT: Local.is_racy lc1_tgt gl1_tgt loc to Ordering.strong_relaxed)
+      (LOCAL1: sim_local lc1_src lc1_tgt)
+      (GLOBAL1: sim_global gl1_src gl1_tgt)
+      (LC_WF1_SRC: Local.wf lc1_src gl1_src)
+      (LC_WF1_TGT: Local.wf lc1_tgt gl1_tgt)
+      (GL_WF1_SRC: Global.wf gl1_src)
+      (GL_WF1_TGT: Global.wf gl1_tgt):
+  <<STEP_SRC: Local.is_racy lc1_src gl1_src loc to Ordering.acqrel>>.
+Proof.
+  exploit sim_local_is_racy;
+    try exact LOCAL1; try exact GLOBAL1; try refl; eauto. i. des.
+  inv x0; eauto.
 Qed.
 
 Lemma sim_local_racy_write_released
-      lc1_src sc1_src mem1_src
-      lc1_tgt sc1_tgt mem1_tgt
+      lc1_src gl1_src
+      lc1_tgt gl1_tgt
       loc to
-      (STEP_TGT: Local.racy_write_step lc1_tgt mem1_tgt loc to Ordering.strong_relaxed)
-      (LOCAL1: sim_local SimPromises.bot lc1_src lc1_tgt)
-      (SC1: TimeMap.le sc1_src sc1_tgt)
-      (MEM1: sim_memory mem1_src mem1_tgt)
-      (WF1_SRC: Local.wf lc1_src mem1_src)
-      (WF1_TGT: Local.wf lc1_tgt mem1_tgt)
-      (SC1_SRC: Memory.closed_timemap sc1_src mem1_src)
-      (SC1_TGT: Memory.closed_timemap sc1_tgt mem1_tgt)
-      (MEM1_SRC: Memory.closed mem1_src)
-      (MEM1_TGT: Memory.closed mem1_tgt):
-  <<STEP_SRC: Local.racy_write_step lc1_src mem1_src loc to Ordering.acqrel>>.
+      (STEP_TGT: Local.racy_write_step lc1_tgt gl1_tgt loc to Ordering.strong_relaxed)
+      (LOCAL1: sim_local lc1_src lc1_tgt)
+      (GLOBAL1: sim_global gl1_src gl1_tgt)
+      (LC_WF1_SRC: Local.wf lc1_src gl1_src)
+      (LC_WF1_TGT: Local.wf lc1_tgt gl1_tgt)
+      (GL_WF1_SRC: Global.wf gl1_src)
+      (GL_WF1_TGT: Global.wf gl1_tgt):
+  <<STEP_SRC: Local.racy_write_step lc1_src gl1_src loc to Ordering.acqrel>>.
 Proof.
-  exploit sim_local_racy_write; try exact STEP_TGT;
-    try exact LOCAL1; try exact SC1; try exact MEM1; try refl; eauto. i. des.
-  inv x0. econs; eauto.
-  inv RACE. econs; eauto.
+  inv STEP_TGT.
+  exploit sim_local_is_racy_released; eauto.
 Qed.
 
 Lemma sim_local_racy_update_released
-      lc1_src sc1_src mem1_src
-      lc1_tgt sc1_tgt mem1_tgt
+      lc1_src gl1_src
+      lc1_tgt gl1_tgt
       loc to ordr
-      (STEP_TGT: Local.racy_update_step lc1_tgt mem1_tgt loc to ordr Ordering.strong_relaxed)
-      (LOCAL1: sim_local SimPromises.bot lc1_src lc1_tgt)
-      (SC1: TimeMap.le sc1_src sc1_tgt)
-      (MEM1: sim_memory mem1_src mem1_tgt)
-      (WF1_SRC: Local.wf lc1_src mem1_src)
-      (WF1_TGT: Local.wf lc1_tgt mem1_tgt)
-      (SC1_SRC: Memory.closed_timemap sc1_src mem1_src)
-      (SC1_TGT: Memory.closed_timemap sc1_tgt mem1_tgt)
-      (MEM1_SRC: Memory.closed mem1_src)
-      (MEM1_TGT: Memory.closed mem1_tgt):
-  <<STEP_SRC: Local.racy_update_step lc1_src mem1_src loc to ordr Ordering.acqrel>>.
+      (STEP_TGT: Local.racy_update_step lc1_tgt gl1_tgt loc to ordr Ordering.strong_relaxed)
+      (LOCAL1: sim_local lc1_src lc1_tgt)
+      (GLOBAL1: sim_global gl1_src gl1_tgt)
+      (LC_WF1_SRC: Local.wf lc1_src gl1_src)
+      (LC_WF1_TGT: Local.wf lc1_tgt gl1_tgt)
+      (GL_WF1_SRC: Global.wf gl1_src)
+      (GL_WF1_TGT: Global.wf gl1_tgt):
+  <<STEP_SRC: Local.racy_update_step lc1_src gl1_src loc to ordr Ordering.acqrel>>.
 Proof.
-  exploit sim_local_racy_update; try exact STEP_TGT;
-    try exact LOCAL1; try exact SC1; try exact MEM1; try refl; eauto. i. des.
+  exploit sim_local_racy_update;
+    try exact LOCAL1; try exact GLOBAL1; try refl; eauto. i. des.
   inv x0.
   - econs 1; eauto.
   - econs 2; eauto.
